Nemonuri/PropositionalLogics/Decidable.lean
@@ -1,0 +1,33 @@
+module
+
+public import Nemonuri.PropositionalLogics.Basic
+
+@[expose] public section
+
+set_option autoImplicit false
+
+namespace Nemonuri.PropositionalLogics
+
+namespace SatRel
+
+variable {E AP: Type*} [Fintype AP] [EvalLike E AP]
+
+open Indicator
+
+theorem defaultAt_isSat_iff {μ: E} {Φ: Formula AP}
+  : (μ ⊨ₚ Φ) ↔ (evalFormulaToBool μ Φ = .true) := by
+  dsimp [IsSat]
+  conv =>
+    lhs; dsimp [DFunLike.coe, defaultAt, Inhabited.default, SatRel.default]; rw [← AreEvalToTrue.eq_true_iff]
+  rfl
+
+instance {μ: E} {Φ: Formula AP} : Decidable (μ ⊨ₚ Φ) := decidable_of_iff' (evalFormulaToBool μ Φ = .true) defaultAt_isSat_iff
+
+
+end SatRel
+
+
+
+end Nemonuri.PropositionalLogics
+
+end
